formic_site_duct/obj/Debug/net6.0/Demo1.AssemblyInfo.cs
@@ -13,7 +13,7 @@ using System.Reflection;
 [assembly: System.Reflection.AssemblyCompanyAttribute("Demo1")]
 [assembly: System.Reflection.AssemblyConfigurationAttribute("Debug")]
 [assembly: System.Reflection.AssemblyFileVersionAttribute("1.0.0.0")]
-[assembly: System.Reflection.AssemblyInformationalVersionAttribute("1.0.0+3c5f8c034d9fd095248747e0e0114ebae9adb0e5")]
+[assembly: System.Reflection.AssemblyInformationalVersionAttribute("1.0.0+34c9ee2b4787f6633863790902ef957370c18f7c")]
 [assembly: System.Reflection.AssemblyProductAttribute("Demo1")]
 [assembly: System.Reflection.AssemblyTitleAttribute("Demo1")]
 [assembly: System.Reflection.AssemblyVersionAttribute("1.0.0.0")]
