formic_site_duct/formic.apis.duct.dfy
@@ -1,5 +1,6 @@
 module DuctApis {
 
+    import opened DB
     import opened DuctImpl
     import opened DuctTools
 
@@ -7,6 +8,7 @@ module DuctApis {
         static method Endpoints() returns (all: AllApiEndpoints)
         {
             var catalog := new AllApiEndpoints();
+            var appDb := new Database();
 
             var formic_landing := new FormicLandingPage();
             var home := new ApiEndpoint("/", ReturnType.Content(""), formic_landing);
@@ -15,6 +17,11 @@ module DuctApis {
             var login_page := new LoginChallengePage();
             var login := new ApiEndpoint("/login", ReturnType.ChallengeGoogle("/"), login_page);
             catalog.Add(login);
+
+            var save_user_page := new SaveUserPage();
+            save_user_page.SetDb(appDb);
+            var save_user := new ApiEndpoint("/save_user", ReturnType.Content(""), save_user_page);
+            catalog.Add(save_user);
 
             var secure_page := new SecurePage();
             var secure := new ApiEndpoint("/secure", ReturnType.Content(""), secure_page);
